

Speaking the Syntax

Ex 1: \leq

Inductive $le : nat \rightarrow nat \rightarrow Prop$ $:=$

| le_n ($n : nat$) $: le\ n\ n$
constructor #1

le_n says: Provided n , we can say $n \leq n$

| le_S ($n\ m : nat$) ($H : le\ n\ m$) $: le\ n\ (S\ m)$
constructor #2

le_S says:

Provided $n \leq m$, we can say $n \leq S\ m$

Ex 2: Collatz

Inductive $Collatz_holds_for : nat \rightarrow Prop$ $:=$

| Chf_done $: Collatz_holds_for\ 2$

| Chf_move ($m : nat$) $: Collatz_holds_for\ (f\ m) \rightarrow$
 $Collatz_holds_for\ m$

or, equivalently,

Inductive $Collatz_holds_for : nat \rightarrow Prop$ $:=$

$Chf_done : Collatz_holds_for\ 2$

$| \text{chf_done} : \text{Collatz_holds_for } 1$
 $| \text{chf_move } (m:\text{nat}) (H: \text{Collatz_holds_for } (f\ m)) :$
 $\text{Collatz_holds_for } m$

The ability to move H in-n-out
 suggests that Chf_move is essentially
 a function.

Let's speak it:

Inductive $\text{Collatz_holds_for} : \text{nat} \rightarrow \text{Prop} :=$

$| \text{chf_done} : \text{Collatz_holds_for } 1$

chf_done says: Collatz holds for 1.

$| \text{chf_move } (m:\text{nat}) (H: \text{Collatz_holds_for } (f\ m)) :$

$\text{Collatz_holds_for } m$

chf_move says: Given m and that Collatz
 holds for $(f\ m)$, we know Collatz holds for m .

Ex 3:

Inductive $\text{Perm3} : [x] \rightarrow [x] \rightarrow \text{Prop} :=$

$| \text{swap12 } (a\ b\ c : x) :$

$\text{Perm3 } [a; b; c] [b; a; c]$

swap12 says: $[a\ b\ c]$ is Perm3 of $[b\ a\ c]$

| swap23 (a b c : X) :
Perm3 [a; b; c] [a; c; b]

swap23 says: [a b c] is perm3 of [a c b]

| trans (l1 l2 l3 : [X]) :

Perm3 l1 l2 → Perm3 l2 l3
→ Perm l1 l3

If l1, l2 are perms and l2, l3 perms,
then l1, l3 are perms.

Inverting on evidences

Evidences are inductive propositions in the hypothesis.

Consider **ev 2** is in the hypothesis, we
should be able to infer?

Of course, we can compute

ev-ss 2 (ev 2) = ev 4

But more interestingly, we should be able
to infer

ev 0

I.e., $ev\ 2 \rightarrow ev\ 0$ via inversion.

Let's do more inversions:

- $ev\ 1 \rightarrow False$

↳ Inverting an improbable construction turns it into False!

- $[n; m] = [0; 0] \rightarrow n=0, m=0$

though inversion is the primary use, inversion also does injection. It actually does quite a lot more.

- $ev\ n \rightarrow \underbrace{n=0}_{\text{corresponds to } ev_0} \quad \backslash /$

$\underbrace{ev\ (n-2)}_{\text{corresponds to } ev_SS}$

- $ev\ (2+n) \rightarrow ev\ n$

- $2 \leq 1 \rightarrow False$

Internally, `coq` is trying to find a 'le' constructor that satisfies $2 \leq 1$:

Can $2 \leq 1$ be `le_n`? No.

Can $2 \leq 1$ be `le_S`? Yes but if only $2 \leq 0$ is `le`.

Can $2 \leq 0$ be le_n ? No.

Can $2 \leq 0$ be le_S ? No.

↖ No because we can't
continue to decrement 0.

$$\bullet \quad S\ n \leq 1 \rightarrow S\ n = 1 \quad \checkmark$$

$$S\ n \leq 0$$

Inducting on inductive props

The tricky stuff!

As we know, induction is destruct plus
assuming previous case, so let's work through
destruct first.

Ex 1

$n: \text{nat}$

$E: \text{ev } n$

(1/1) Goal

Even n

after destruct E

$n: \text{nat}$

$E: \text{ev } n'$

(1/2) Goal

Even 0

(2/2) Goal

Even $(2 + n')$

What's going on?

Recall that inverting $\text{ev } n$ gives

$n = 0 \quad \vee \quad \text{ev } (n - 2)$

So, • in the first case, $n = 0$, hence $\text{Even} = 0$.

• in the second case, $\text{ev } (n - 2)$ means that there is a $n' = n - 2$ such that $\text{ev } n'$.

The new variable n' is used to rewrite all hypotheses and the goal.

added
as
hypothesis.

Hence, $\text{Even } n$ becomes $\text{Even } (2 + n')$

now, what about induction?

$n: \text{nat}$

$E: \text{ev } n$

(1/1) Goal

Even n

after induction E

n : nat

E : ev n'

H : Even n' \rightarrow the only difference!

(1/2) Goal

Even 0

(2/2) Goal

Even $(2 + n')$

okay. Why are we able to infer Even n' ?

Ex 2

m, n, o : nat

H : $m \leq n$

H_0 : $n \leq o$

(1/1)

$m \leq o$

After induction $[n \leq 0]$:

$m, n : \text{nat}$

$H : m \leq n$

(1/2)

$m \leq n$

\downarrow
0 got replaced by n.

$m, n : \text{nat}$

$H : m \leq n$

$o' : \text{nat}$

$Hno' : n \leq o'$

$IHmo' : m \leq o'$

(2/2)

$m \leq S o'$

$n \leq 0$ either means

- le_n , in which case n matches the argument, and we must have $0 = n$ to get $n \leq n$.

- le_S , in which case we must have

$n \leq o'$, where $0 = o' + 1$

$o' = 0 - 1$

$$H: a > b$$

✓

case gt_base : a matches, and

$$S a' > a'$$

$$a' = a - 1, \quad b = a'$$

$$H_0: a' > c$$

$$G: S a' > c$$

case gt_S : a, b matches with n, m ,

$$a > b \quad \Leftrightarrow \quad (n+2) > (m+1)$$

$$\boxed{\begin{array}{l} a = n+2 \\ b = m+1 \end{array}}$$

$H_0: b > c$ becomes

$$m+1 > c$$

G: $A > C$ becomes

$$n+2 > C$$